veric/semax_conseq.v
@@ -57,14 +57,14 @@ Proof.
   apply _guard_mono; auto.
 Qed.
 
-Definition bupd_ret_assert (Q: ret_assert): ret_assert :=
-          {| RA_normal := fun rho => bupd (RA_normal Q rho);
-             RA_break := fun rho => bupd (RA_break Q rho);
-             RA_continue := fun rho => bupd (RA_continue Q rho);
-             RA_return := fun v rho => bupd (RA_return Q v rho) |}.
+Definition fupd_ret_assert (Q: ret_assert): ret_assert :=
+          {| RA_normal := fun rho => fupd (RA_normal Q rho);
+             RA_break := fun rho => fupd (RA_break Q rho);
+             RA_continue := fun rho => fupd (RA_continue Q rho);
+             RA_return := fun v rho => fupd (RA_return Q v rho) |}.
 
-Lemma bupd_andp_prop:
-  forall P Q, bupd (!! P && Q) = !!P && bupd Q.
+Lemma fupd_andp_prop:
+  forall P Q, fupd (!! P && Q) = !!P && fupd Q.
 Proof.
 intros.
 apply pred_ext; repeat intro.
@@ -82,26 +82,26 @@ rewrite prop_true_andp in * by auto.
 auto.
 Qed.
 
-Lemma proj_bupd_ret_assert: forall Q ek vl,
-  proj_ret_assert (bupd_ret_assert Q) ek vl = fun rho => bupd (proj_ret_assert Q ek vl rho).
+Lemma proj_fupd_ret_assert: forall Q ek vl,
+  proj_ret_assert (fupd_ret_assert Q) ek vl = fun rho => fupd (proj_ret_assert Q ek vl rho).
 Proof.
   intros.
  extensionality rho.
   destruct ek; simpl; auto;
-  rewrite bupd_andp_prop; auto.
+  rewrite fupd_andp_prop; auto.
 Qed.
 
 (* The following four lemmas is not now used. but after deep embedded hoare logic (SL_as_Logic) is
 ported, the frame does not need to be quantified in the semantic definition of semax. Then,
 these two lemmas can replace the other two afterwards. *)
 
-Lemma assert_safe_bupd':
+Lemma assert_safe_fupd':
   forall {Espec: OracleKind} gx vx tx rho (P: environ -> pred rmap) Delta f k,
     let PP1 := !! guard_environ Delta f rho in
     let PP2 := funassert Delta rho in
     PP1 && (P rho) && PP2 >=>
     assert_safe Espec gx f vx tx k rho =
-    PP1 && (bupd (P rho)) && PP2 >=>
+    PP1 && (fupd (P rho)) && PP2 >=>
     assert_safe Espec gx f vx tx k rho.
 Proof.
   intros.
@@ -110,7 +110,7 @@ Proof.
     hnf; intros.
     intros ?? H1 Hext H2.
     destruct H2 as [[? ?] ?].
-    apply bupd_trans.
+    apply fupd_trans.
     hnf.
     intros.
     specialize (H3 _ H5).
@@ -130,47 +130,47 @@ Proof.
     eapply H; eauto.
     destruct H2 as [[? ?] ?].
     split; [split |]; auto.
-    apply bupd_intro; auto.
+    apply fupd_intro; auto.
 Qed.
 
-Lemma _guard_bupd':
+Lemma _guard_fupd':
   forall {Espec: OracleKind} ge Delta (P: environ -> pred rmap) f k,
-    _guard Espec ge Delta f P k = _guard Espec ge Delta f (fun rho => bupd (P rho)) k.
+    _guard Espec ge Delta f P k = _guard Espec ge Delta f (fun rho => fupd (P rho)) k.
 Proof.
   intros.
   unfold _guard.
   f_equal; extensionality tx.
   f_equal; extensionality vx.
-  apply assert_safe_bupd'.
+  apply assert_safe_fupd'.
 Qed.
   
-Lemma guard_bupd':
+Lemma guard_fupd':
   forall {Espec: OracleKind} ge Delta f (P: environ -> pred rmap) k,
-    guard Espec ge Delta f P k = guard Espec ge Delta f (fun rho => bupd (P rho)) k.
+    guard Espec ge Delta f P k = guard Espec ge Delta f (fun rho => fupd (P rho)) k.
 Proof.
   intros.
-  apply _guard_bupd'.
+  apply _guard_fupd'.
 Qed.
 
-Lemma rguard_bupd':
+Lemma rguard_fupd':
   forall {Espec: OracleKind} ge Delta f (P: ret_assert) k,
-    rguard Espec ge Delta f P k = rguard Espec ge Delta f (bupd_ret_assert P) k.
+    rguard Espec ge Delta f P k = rguard Espec ge Delta f (fupd_ret_assert P) k.
 Proof.
   intros.
   unfold rguard.
   f_equal; extensionality ek.
   f_equal; extensionality vl.
-  rewrite proj_bupd_ret_assert.
-  apply _guard_bupd'.
+  rewrite proj_fupd_ret_assert.
+  apply _guard_fupd'.
 Qed.
 
-Lemma assert_safe_bupd:
+Lemma assert_safe_fupd:
   forall {Espec: OracleKind} gx vx tx rho (F P: environ -> pred rmap) Delta f k,
     let PP1 := !! guard_environ Delta f rho in
     let PP2 := funassert Delta rho in
     PP1 && (F rho * P rho) && PP2 >=>
     assert_safe Espec gx f vx tx k rho =
-    PP1 && (F rho * bupd (P rho)) && PP2 >=>
+    PP1 && (F rho * fupd (P rho)) && PP2 >=>
     assert_safe Espec gx f vx tx k rho.
 Proof.
   intros.
@@ -179,10 +179,10 @@ Proof.
     hnf; intros.
     intros ?? H1 Hext H2.
     destruct H2 as [[? ?] ?].
-    apply bupd_trans.
+    apply fupd_trans.
     hnf.
     intros.
-    apply bupd_frame_l in H3.
+    apply fupd_frame_l in H3.
     specialize (H3 _ H5).
     destruct H3 as [b [? [m' [? [? [? ?]]]]]].
     exists b; split; auto.
@@ -202,39 +202,39 @@ Proof.
     split; [split |]; auto.
     revert H3.
     apply sepcon_derives; auto.
-    apply bupd_intro.
+    apply fupd_intro.
 Qed.
 
-Lemma _guard_bupd:
+Lemma _guard_fupd:
   forall {Espec: OracleKind} ge Delta f (F P: environ -> pred rmap) k,
-    _guard Espec ge Delta f (fun rho => F rho * P rho) k = _guard Espec ge Delta f (fun rho => F rho * bupd (P rho)) k.
+    _guard Espec ge Delta f (fun rho => F rho * P rho) k = _guard Espec ge Delta f (fun rho => F rho * fupd (P rho)) k.
 Proof.
   intros.
   unfold _guard.
   f_equal; extensionality tx.
   f_equal; extensionality vx.
-  apply assert_safe_bupd.
+  apply assert_safe_fupd.
 Qed.
   
-Lemma guard_bupd:
+Lemma guard_fupd:
   forall {Espec: OracleKind} ge Delta f (F P: environ -> pred rmap) k,
-    guard Espec ge Delta f (fun rho => F rho * P rho) k = guard Espec ge Delta f (fun rho => F rho * bupd (P rho)) k.
+    guard Espec ge Delta f (fun rho => F rho * P rho) k = guard Espec ge Delta f (fun rho => F rho * fupd (P rho)) k.
 Proof.
   intros.
-  apply _guard_bupd.
+  apply _guard_fupd.
 Qed.
 
-Lemma rguard_bupd:
+Lemma rguard_fupd:
   forall {Espec: OracleKind} ge Delta F f (P: ret_assert) k,
-    rguard Espec ge Delta f (frame_ret_assert P F) k = rguard Espec ge Delta f (frame_ret_assert (bupd_ret_assert P) F) k.
+    rguard Espec ge Delta f (frame_ret_assert P F) k = rguard Espec ge Delta f (frame_ret_assert (fupd_ret_assert P) F) k.
 Proof.
   intros.
   unfold rguard.
   f_equal; extensionality ek.
   f_equal; extensionality vl.
   rewrite !proj_frame.
-  rewrite proj_bupd_ret_assert.
-  apply _guard_bupd.
+  rewrite proj_fupd_ret_assert.
+  apply _guard_fupd.
 Qed.
 
 Definition except_0_ret_assert (Q: ret_assert): ret_assert :=
@@ -539,15 +539,15 @@ Qed.
 Lemma semax_conseq {CS: compspecs} {Espec: OracleKind}:
  forall Delta P' (R': ret_assert) P c (R: ret_assert) ,
    (forall rho,  seplog.derives (!!(typecheck_environ Delta rho) && (allp_fun_id Delta rho && P rho))
-                   (bupd (|> FF || P' rho)) ) ->
+                   (fupd (|> FF || P' rho)) ) ->
    (forall rho,  seplog.derives (!!(typecheck_environ Delta rho) && (allp_fun_id Delta rho && RA_normal R' rho))
-                   (bupd (|> FF || RA_normal R rho))) ->
+                   (fupd (|> FF || RA_normal R rho))) ->
    (forall rho, seplog.derives (!! (typecheck_environ Delta rho) && (allp_fun_id Delta rho && RA_break R' rho))
-                   (bupd (|> FF || RA_break R rho))) ->
+                   (fupd (|> FF || RA_break R rho))) ->
    (forall rho, seplog.derives (!! (typecheck_environ Delta rho) && (allp_fun_id Delta rho && RA_continue R' rho))
-                   (bupd (|> FF || RA_continue R rho))) ->
+                   (fupd (|> FF || RA_continue R rho))) ->
    (forall vl rho, seplog.derives (!! (typecheck_environ Delta rho) && (allp_fun_id Delta rho && RA_return R' vl rho))
-                   (bupd (|> FF || RA_return R vl rho))) ->
+                   (fupd (|> FF || RA_return R vl rho))) ->
    semax Espec Delta P' c R' ->  semax Espec Delta P c R.
 Proof.
   intros.
@@ -566,11 +566,11 @@ Proof.
  + erewrite (rguard_allp_fun_id _ _ _ _ _ R') by eauto.
     erewrite (rguard_tc_environ _ _ _ _ _ (conj_ret_assert R' _)) by eauto.
     eapply derives_trans; [apply  (rguard_except_0 _ _ _ _ R) |].
-    rewrite (rguard_bupd _ _ _ _ (except_0_ret_assert _)).
+    rewrite (rguard_fupd _ _ _ _ (except_0_ret_assert _)).
     apply rguard_mono.
     intros.
     rewrite proj_frame, proj_conj, proj_conj.
-    rewrite proj_frame, proj_bupd_ret_assert.
+    rewrite proj_frame, proj_fupd_ret_assert.
     apply sepcon_derives; auto.
     destruct rk;
          [rename H0 into Hx; pose (ek:=RA_normal)
@@ -587,7 +587,7 @@ all:    specialize (Hx rho); inv Hx; simpl in *;
   + erewrite (guard_allp_fun_id _ _ _ _ _ P) by eauto.
     erewrite (guard_tc_environ _ _ _ _ _ (fun rho => allp_fun_id Delta rho && P rho)) by eauto.
     rewrite (guard_except_0 _ _ _ _ P').
-    rewrite (guard_bupd _ _ _ _ (fun rho => |> FF || P' rho)).
+    rewrite (guard_fupd _ _ _ _ (fun rho => |> FF || P' rho)).
     apply guard_mono.
     intros.
     apply sepcon_derives; auto.
@@ -595,11 +595,11 @@ all:    specialize (Hx rho); inv Hx; simpl in *;
 Qed.
 
 (* Part 2: Deriving simpler and older version of consequence rules from semax_conseq. *)
-Lemma semax'_post_bupd:
+Lemma semax'_post_fupd:
  forall {CS: compspecs} {Espec: OracleKind} (R': ret_assert) Delta (R: ret_assert) P c,
    (forall ek vl rho,  !!(typecheck_environ Delta rho ) && 
                 proj_ret_assert R' ek vl rho 
-         |-- bupd (proj_ret_assert R ek vl rho)) ->
+         |-- fupd (proj_ret_assert R ek vl rho)) ->
    semax' Espec Delta P c R' |-- semax' Espec Delta P c R.
 Proof.
 intros.
@@ -622,7 +622,7 @@ apply allp_derives; intro ve.
 intros ? ?.
 intros ? ? ? ? ? Hext ?.
 destruct H3 as [[? HFP] ?].
-assert (bupd (proj_ret_assert (frame_ret_assert R F) ek vl
+assert (fupd (proj_ret_assert (frame_ret_assert R F) ek vl
   (construct_rho (filter_genv psi) ve te)) a'') as HFP'.
 { specialize (H ek vl (construct_rho (filter_genv psi) ve te)).
   rewrite prop_true_andp in H.
@@ -632,26 +632,26 @@ assert (bupd (proj_ret_assert (frame_ret_assert R F) ek vl
     destruct HFP as [Hvl HFP]. rewrite !prop_true_andp in H by auto.
     simpl proj_ret_assert. rewrite prop_true_andp by auto.
     eapply sepcon_derives in HFP; [| apply H | apply derives_refl].
-    apply bupd_frame_r in HFP.
+    apply fupd_frame_r in HFP.
     destruct R; auto.
   * destruct R'.
     destruct HFP as [Hvl HFP]. rewrite !prop_true_andp in H by auto.
     simpl proj_ret_assert. rewrite prop_true_andp by auto.
     eapply sepcon_derives in HFP; [| apply H | apply derives_refl].
-    apply bupd_frame_r in HFP.
+    apply fupd_frame_r in HFP.
     destruct R; auto.
   * destruct R'.
     destruct HFP as [Hvl HFP]. rewrite !prop_true_andp in H by auto.
     simpl proj_ret_assert. rewrite prop_true_andp by auto.
     eapply sepcon_derives in HFP; [| apply H | apply derives_refl].
-    apply bupd_frame_r in HFP.
+    apply fupd_frame_r in HFP.
     destruct R; auto.
   * destruct R'.
     eapply sepcon_derives in HFP; [| apply H | apply derives_refl].
-    apply bupd_frame_r in HFP.
+    apply fupd_frame_r in HFP.
     destruct R; auto.
   * destruct H3; eapply typecheck_environ_sub; eauto. }
-assert ((bupd (assert_safe Espec psi f ve te (exit_cont ek vl k)
+assert ((fupd (assert_safe Espec psi f ve te (exit_cont ek vl k)
   (construct_rho (filter_genv psi) ve te))) a'') as Hsafe.
 { intros ? J.
   destruct (HFP' _ J) as (b & ? & m' & ? & ? & ? & ?).
@@ -662,7 +662,7 @@ assert ((bupd (assert_safe Espec psi f ve te (exit_cont ek vl k)
   intro X; eapply X; auto.
   split; [split|]; auto.
   apply funassert_resource with (a := a''); auto. }
-eapply bupd_trans; eauto.
+eapply fupd_trans; eauto.
 Qed.
 
 Lemma semax'_post:
@@ -673,13 +673,13 @@ Lemma semax'_post:
    semax' Espec Delta P c R' |-- semax' Espec Delta P c R.
 Proof.
 intros.
-apply semax'_post_bupd.
-intros; eapply derives_trans, bupd_intro; auto.
+apply semax'_post_fupd.
+intros; eapply derives_trans, fupd_intro; auto.
 Qed.
 
-Lemma semax'_pre_bupd:
+Lemma semax'_pre_fupd:
  forall {CS: compspecs} {Espec: OracleKind} P' Delta R P c,
-  (forall rho, typecheck_environ Delta rho ->   P rho |-- bupd (P' rho))
+  (forall rho, typecheck_environ Delta rho ->   P rho |-- fupd (P' rho))
    ->   semax' Espec Delta P' c R |-- semax' Espec Delta P c R.
 Proof.
 intros.
@@ -700,8 +700,8 @@ intros ? ?.
 intros ? ? ? ? ? Hext ?.
 destruct H3 as [[? HFP] ?].
 eapply sepcon_derives in HFP; [| apply derives_refl | apply H].
-apply bupd_frame_l in HFP.
-apply bupd_trans; intros ? J.
+apply fupd_frame_l in HFP.
+apply fupd_trans; intros ? J.
 destruct (HFP _ J) as (b & ? & m' & ? & ? & ? & HFP').
 exists b; split; auto; exists m'; repeat split; auto.
 pose proof (necR_level _ _ H2).
@@ -718,23 +718,23 @@ Lemma semax'_pre:
   (forall rho, typecheck_environ Delta rho ->   P rho |-- P' rho)
    ->   semax' Espec Delta P' c R |-- semax' Espec Delta P c R.
 Proof.
-intros; apply semax'_pre_bupd.
-intros; eapply derives_trans, bupd_intro; auto.
+intros; apply semax'_pre_fupd.
+intros; eapply derives_trans, fupd_intro; auto.
 Qed.
 
-Lemma semax'_pre_post_bupd:
+Lemma semax'_pre_post_fupd:
  forall
       {CS: compspecs} {Espec: OracleKind} P' (R': ret_assert) Delta (R: ret_assert) P c,
-   (forall rho, typecheck_environ Delta rho ->   P rho |-- bupd (P' rho)) ->
+   (forall rho, typecheck_environ Delta rho ->   P rho |-- fupd (P' rho)) ->
    (forall ek vl rho, !!(typecheck_environ Delta rho) 
                        &&  proj_ret_assert R ek vl rho 
-                    |-- bupd (proj_ret_assert R' ek vl rho)) ->
+                    |-- fupd (proj_ret_assert R' ek vl rho)) ->
    semax' Espec Delta P' c R |-- semax' Espec Delta P c R'.
 Proof.
 intros.
 eapply derives_trans.
-apply semax'_pre_bupd; eauto.
-apply semax'_post_bupd; auto.
+apply semax'_pre_fupd; eauto.
+apply semax'_post_fupd; auto.
 Qed.
 
 Lemma semax'_pre_post:
@@ -752,36 +752,36 @@ apply semax'_pre; eauto.
 apply semax'_post; auto.
 Qed.
 
-Lemma semax_post'_bupd {CS: compspecs} {Espec: OracleKind}:
+Lemma semax_post'_fupd {CS: compspecs} {Espec: OracleKind}:
  forall (R': ret_assert) Delta (R: ret_assert) P c,
    (forall ek vl rho,  !!(typecheck_environ Delta rho) 
                       &&  proj_ret_assert R' ek vl rho
-                        |-- bupd (proj_ret_assert R ek vl rho)) ->
+                        |-- fupd (proj_ret_assert R ek vl rho)) ->
    semax Espec Delta P c R' ->  semax Espec Delta P c R.
 Proof.
 unfold semax.
 intros.
 specialize (H0 n). revert n H0.
-apply semax'_post_bupd.
+apply semax'_post_fupd.
 auto.
 Qed.
 
-Lemma semax_post_bupd {CS: compspecs} {Espec: OracleKind}:
+Lemma semax_post_fupd {CS: compspecs} {Espec: OracleKind}:
  forall (R': ret_assert) Delta (R: ret_assert) P c,
    (forall rho,  !!(typecheck_environ Delta rho) 
-                      &&  RA_normal R' rho |-- bupd (RA_normal R rho)) ->
+                      &&  RA_normal R' rho |-- fupd (RA_normal R rho)) ->
    (forall rho, !! (typecheck_environ Delta rho) 
-                      && RA_break R' rho |-- bupd (RA_break R rho)) ->
+                      && RA_break R' rho |-- fupd (RA_break R rho)) ->
    (forall rho, !! (typecheck_environ Delta rho) 
-                      && RA_continue R' rho |-- bupd (RA_continue R rho)) ->
+                      && RA_continue R' rho |-- fupd (RA_continue R rho)) ->
    (forall vl rho, !! (typecheck_environ Delta rho) 
-                      && RA_return R' vl rho |-- bupd (RA_return R vl rho)) ->
+                      && RA_return R' vl rho |-- fupd (RA_return R vl rho)) ->
    semax Espec Delta P c R' ->  semax Espec Delta P c R.
 Proof.
 unfold semax.
 intros.
 specialize (H3 n). revert n H3.
-apply semax'_post_bupd.
+apply semax'_post_fupd.
 intros; destruct ek; simpl;
 repeat (apply normalize.derives_extract_prop; intro); rewrite ?prop_true_andp by auto;
 specialize (H rho); specialize (H0 rho); specialize (H1 rho); specialize (H2 vl rho);
@@ -824,16 +824,16 @@ specialize (H rho); specialize (H0 rho); specialize (H1 rho); specialize (H2 vl 
 rewrite prop_true_andp in H, H0, H1, H2 by auto; auto.
 Qed.
 
-Lemma semax_pre_bupd {CS: compspecs} {Espec: OracleKind} :
+Lemma semax_pre_fupd {CS: compspecs} {Espec: OracleKind} :
  forall P' Delta P c R,
-   (forall rho,  !!(typecheck_environ Delta rho) &&  P rho |-- bupd (P' rho) )%pred ->
+   (forall rho,  !!(typecheck_environ Delta rho) &&  P rho |-- fupd (P' rho) )%pred ->
      semax Espec Delta P' c R  -> semax Espec Delta P c R.
 Proof.
 unfold semax.
 intros.
 specialize (H0 n).
 revert n H0.
-apply semax'_pre_bupd.
+apply semax'_pre_fupd.
 repeat intro. apply (H rho a); auto. split; auto.
 Qed.
 
@@ -850,22 +850,22 @@ apply semax'_pre.
 repeat intro. apply (H rho a). split; auto.
 Qed.
 
-Lemma semax_pre_post_bupd {CS: compspecs} {Espec: OracleKind}:
+Lemma semax_pre_post_fupd {CS: compspecs} {Espec: OracleKind}:
  forall P' (R': ret_assert) Delta P c (R: ret_assert) ,
-   (forall rho,  !!(typecheck_environ Delta rho) &&  P rho |-- bupd (P' rho) )%pred ->
+   (forall rho,  !!(typecheck_environ Delta rho) &&  P rho |-- fupd (P' rho) )%pred ->
    (forall rho,  !!(typecheck_environ Delta rho) 
-                      &&  RA_normal R' rho |-- bupd (RA_normal R rho)) ->
+                      &&  RA_normal R' rho |-- fupd (RA_normal R rho)) ->
    (forall rho, !! (typecheck_environ Delta rho) 
-                      && RA_break R' rho |-- bupd (RA_break R rho)) ->
+                      && RA_break R' rho |-- fupd (RA_break R rho)) ->
    (forall rho, !! (typecheck_environ Delta rho) 
-                      && RA_continue R' rho |-- bupd (RA_continue R rho)) ->
+                      && RA_continue R' rho |-- fupd (RA_continue R rho)) ->
    (forall vl rho, !! (typecheck_environ Delta rho) 
-                      && RA_return R' vl rho |-- bupd (RA_return R vl rho)) ->
+                      && RA_return R' vl rho |-- fupd (RA_return R vl rho)) ->
    semax Espec Delta P' c R' ->  semax Espec Delta P c R.
 Proof.
 intros.
-eapply semax_pre_bupd; eauto.
-eapply semax_post_bupd; eauto.
+eapply semax_pre_fupd; eauto.
+eapply semax_post_fupd; eauto.
 Qed.
 
 Lemma semax_pre_post {CS: compspecs} {Espec: OracleKind}:
@@ -886,11 +886,11 @@ eapply semax_pre; eauto.
 eapply semax_post; eauto.
 Qed.
 
-Lemma semax_bupd_elim {CS: compspecs} {Espec: OracleKind}:
+Lemma semax_fupd_elim {CS: compspecs} {Espec: OracleKind}:
  forall Delta P c R,
-  semax Espec Delta P c R -> semax Espec Delta (fun rho => bupd (P rho)) c R.
+  semax Espec Delta P c R -> semax Espec Delta (fun rho => fupd (P rho)) c R.
 Proof.
-intros ????; apply semax_pre_bupd.
+intros ????; apply semax_pre_fupd.
 intro; apply prop_andp_left; auto.
 Qed.
 
@@ -922,82 +922,82 @@ Qed.
 
 Lemma semax_adapt_frame {cs Espec} Delta c (P P': assert) (Q Q' : ret_assert)
    (H: forall rho,  derives (!!(typecheck_environ Delta rho) && (allp_fun_id Delta rho && P rho))
-                   (EX F: assert, (!!(closed_wrt_modvars c F) && bupd (P' rho * F rho) &&
-                         !!(forall rho, (local (tc_environ Delta) rho) && ((allp_fun_id Delta rho)) && RA_normal (frame_ret_assert Q' F) rho |-- bupd (RA_normal Q rho)) &&
-                         !!(forall rho, (local (tc_environ Delta) rho) && ((allp_fun_id Delta rho)) && RA_break (frame_ret_assert Q' F) rho |-- bupd (RA_break Q rho)) &&
-                         !!(forall rho, (local (tc_environ Delta) rho) && ((allp_fun_id Delta rho)) && RA_continue (frame_ret_assert Q' F) rho |-- bupd (RA_continue Q rho)) &&
-                         !!(forall vl rho, (local (tc_environ Delta) rho) && ((allp_fun_id Delta rho)) && RA_return (frame_ret_assert Q' F) vl rho |-- bupd (RA_return Q vl rho)))))
+                   (EX F: assert, (!!(closed_wrt_modvars c F) && fupd (P' rho * F rho) &&
+                         !!(forall rho, (local (tc_environ Delta) rho) && ((allp_fun_id Delta rho)) && RA_normal (frame_ret_assert Q' F) rho |-- fupd (RA_normal Q rho)) &&
+                         !!(forall rho, (local (tc_environ Delta) rho) && ((allp_fun_id Delta rho)) && RA_break (frame_ret_assert Q' F) rho |-- fupd (RA_break Q rho)) &&
+                         !!(forall rho, (local (tc_environ Delta) rho) && ((allp_fun_id Delta rho)) && RA_continue (frame_ret_assert Q' F) rho |-- fupd (RA_continue Q rho)) &&
+                         !!(forall vl rho, (local (tc_environ Delta) rho) && ((allp_fun_id Delta rho)) && RA_return (frame_ret_assert Q' F) vl rho |-- fupd (RA_return Q vl rho)))))
    (SEM: @semax cs Espec Delta P' c Q'):
    @semax cs Espec Delta P c Q.
 Proof. intros.
-apply (semax_conseq Delta (fun rho => EX F: assert, !!(closed_wrt_modvars c F) && (bupd (sepcon (P' rho) (F rho)) &&
-                         (!!(forall rho, (local (tc_environ Delta) rho) && ((allp_fun_id Delta rho)) && RA_normal (frame_ret_assert Q' F) rho |-- bupd (RA_normal Q rho)) &&
-                         (!!(forall rho, (local (tc_environ Delta) rho) && ((allp_fun_id Delta rho)) && RA_break (frame_ret_assert Q' F) rho |-- bupd (RA_break Q rho)) &&
-                         (!!(forall rho, (local (tc_environ Delta) rho) && ((allp_fun_id Delta rho)) && RA_continue (frame_ret_assert Q' F) rho |-- bupd (RA_continue Q rho)) &&
-                         (!!(forall vl rho, (local (tc_environ Delta) rho) && ((allp_fun_id Delta rho)) && RA_return (frame_ret_assert Q' F) vl rho |-- bupd (RA_return Q vl rho))))))))
+apply (semax_conseq Delta (fun rho => EX F: assert, !!(closed_wrt_modvars c F) && (fupd (sepcon (P' rho) (F rho)) &&
+                         (!!(forall rho, (local (tc_environ Delta) rho) && ((allp_fun_id Delta rho)) && RA_normal (frame_ret_assert Q' F) rho |-- fupd (RA_normal Q rho)) &&
+                         (!!(forall rho, (local (tc_environ Delta) rho) && ((allp_fun_id Delta rho)) && RA_break (frame_ret_assert Q' F) rho |-- fupd (RA_break Q rho)) &&
+                         (!!(forall rho, (local (tc_environ Delta) rho) && ((allp_fun_id Delta rho)) && RA_continue (frame_ret_assert Q' F) rho |-- fupd (RA_continue Q rho)) &&
+                         (!!(forall vl rho, (local (tc_environ Delta) rho) && ((allp_fun_id Delta rho)) && RA_return (frame_ret_assert Q' F) vl rho |-- fupd (RA_return Q vl rho))))))))
    Q).
 + intros. eapply seplog.derives_trans. constructor. apply H. clear H.
-  eapply seplog.derives_trans. 2: { constructor. apply own.bupd_intro. }
+  eapply seplog.derives_trans. 2: { constructor. apply own.fupd_intro. }
   constructor. apply orp_right2. apply exp_derives; intros F. 
   rewrite <- ! andp_assoc; trivial.
-+ clear H. intros. constructor. eapply derives_trans. 2: apply own.bupd_intro.
++ clear H. intros. constructor. eapply derives_trans. 2: apply own.fupd_intro.
   apply orp_right2. do 2 apply andp_left2; trivial.
-+ clear H. intros. constructor. eapply derives_trans. 2: apply own.bupd_intro.
++ clear H. intros. constructor. eapply derives_trans. 2: apply own.fupd_intro.
   apply orp_right2. do 2 apply andp_left2; trivial.
-+ clear H. intros. constructor. eapply derives_trans. 2: apply own.bupd_intro.
++ clear H. intros. constructor. eapply derives_trans. 2: apply own.fupd_intro.
   apply orp_right2. do 2 apply andp_left2; trivial.
-+ clear H. intros. constructor. eapply derives_trans. 2: apply own.bupd_intro.
++ clear H. intros. constructor. eapply derives_trans. 2: apply own.fupd_intro.
   apply orp_right2. do 2 apply andp_left2; trivial.
 + apply extract_exists_pre. intros F. clear H.
   apply semax_extract_prop. intros.
-  eapply semax_pre_bupd. 2:{ do 4 (apply semax_extract_prop; intros). 
+  eapply semax_pre_fupd. 2:{ do 4 (apply semax_extract_prop; intros). 
     eapply semax_conseq. 6:{ apply semax_frame. exact H. apply SEM. }
     2: {
-    intros; constructor. eapply derives_trans; [|apply bupd_mono; apply derives_refl].
+    intros; constructor. eapply derives_trans; [|apply fupd_mono; apply derives_refl].
     revert rho. exact H0. }
     2: {
-    intros; constructor. eapply derives_trans; [|apply bupd_mono; apply derives_refl].
+    intros; constructor. eapply derives_trans; [|apply fupd_mono; apply derives_refl].
     revert rho. exact H1. }
     2: {
-    intros; constructor. eapply derives_trans; [|apply bupd_mono; apply derives_refl].
+    intros; constructor. eapply derives_trans; [|apply fupd_mono; apply derives_refl].
     revert rho. exact H2. }
     2: {
-    intros; constructor. eapply derives_trans; [|apply bupd_mono; apply derives_refl].
+    intros; constructor. eapply derives_trans; [|apply fupd_mono; apply derives_refl].
     revert rho. revert vl. exact H3. }
     
   (* 2: { *)
-  (*  intros; constructor. eapply derives_trans; [ | apply own.bupd_intro]. *)
+  (*  intros; constructor. eapply derives_trans; [ | apply own.fupd_intro]. *)
   (*  apply orp_right2. revert rho. exact H1. } *)
   (* 2: { *)
-  (*  intros; constructor. eapply derives_trans; [ | apply own.bupd_intro].  *)
+  (*  intros; constructor. eapply derives_trans; [ | apply own.fupd_intro].  *)
   (*  apply orp_right2. revert rho. revert vl. exact H3. } *)
   
-   intros; constructor. eapply derives_trans; [ | apply own.bupd_intro]. 
+   intros; constructor. eapply derives_trans; [ | apply own.fupd_intro]. 
    apply orp_right2. apply andp_left2. apply andp_left2. apply derives_refl. }
   intros. unfold local, liftx, lift1, tc_environ; simpl. apply andp_left2.
-  rewrite (andp_comm (bupd (P' rho * F rho))). rewrite !bupd_andp_prop.
+  rewrite (andp_comm (fupd (P' rho * F rho))). rewrite !fupd_andp_prop.
   rewrite <- ! andp_assoc. repeat apply andp_derives; auto.
   * apply prop_derives. intros. rewrite <- andp_assoc.
-    apply derives_trans with (bupd (RA_normal Q rho0)); [apply H0|].
-    apply bupd_mono. apply orp_right2; auto.
+    apply derives_trans with (fupd (RA_normal Q rho0)); [apply H0|].
+    apply fupd_mono. apply orp_right2; auto.
   * apply prop_derives. intros. rewrite <- andp_assoc.
-    apply derives_trans with (bupd (RA_break Q rho0)); [apply H0|].
-    apply bupd_mono. apply orp_right2; auto.
+    apply derives_trans with (fupd (RA_break Q rho0)); [apply H0|].
+    apply fupd_mono. apply orp_right2; auto.
   * apply prop_derives. intros. rewrite <- andp_assoc.
-    apply derives_trans with (bupd (RA_continue Q rho0)); [apply H0|].
-    apply bupd_mono. apply orp_right2; auto.
+    apply derives_trans with (fupd (RA_continue Q rho0)); [apply H0|].
+    apply fupd_mono. apply orp_right2; auto.
   * apply prop_derives. intros. rewrite <- andp_assoc.
-    apply derives_trans with (bupd (RA_return Q vl rho0)); [apply H0|].
-    apply bupd_mono. apply orp_right2; auto.
+    apply derives_trans with (fupd (RA_return Q vl rho0)); [apply H0|].
+    apply fupd_mono. apply orp_right2; auto.
 Qed.
 
 Lemma semax_adapt_frame' {cs Espec} Delta c (P P': assert) (Q Q' : ret_assert)
    (H: forall rho,  !!(typecheck_environ Delta rho) && (allp_fun_id Delta rho && P rho)
-                   |-- EX F: assert, (!!(closed_wrt_modvars c F) && bupd (P' rho * F rho) &&
-                        !!(forall rho, RA_normal (frame_ret_assert Q' F) rho |-- bupd (RA_normal Q rho)) &&
-                        !!(forall rho, RA_break (frame_ret_assert Q' F) rho |-- bupd (RA_break Q rho)) &&
-                        !!(forall rho, RA_continue (frame_ret_assert Q' F) rho |-- bupd (RA_continue Q rho)) &&
-                        !!(forall vl rho, RA_return (frame_ret_assert Q' F) vl rho |-- bupd (RA_return Q vl rho))))
+                   |-- EX F: assert, (!!(closed_wrt_modvars c F) && fupd (P' rho * F rho) &&
+                        !!(forall rho, RA_normal (frame_ret_assert Q' F) rho |-- fupd (RA_normal Q rho)) &&
+                        !!(forall rho, RA_break (frame_ret_assert Q' F) rho |-- fupd (RA_break Q rho)) &&
+                        !!(forall rho, RA_continue (frame_ret_assert Q' F) rho |-- fupd (RA_continue Q rho)) &&
+                        !!(forall vl rho, RA_return (frame_ret_assert Q' F) vl rho |-- fupd (RA_return Q vl rho))))
    (SEM: @semax cs Espec Delta P' c Q'):
    @semax cs Espec Delta P c Q.
 Proof.
@@ -1018,11 +1018,11 @@ Qed.
 
 Lemma semax_adapt {cs Espec} Delta c (P P': assert) (Q Q' : ret_assert)
    (H: forall rho,  !!(typecheck_environ Delta rho) && (allp_fun_id Delta rho && P rho)
-                   |-- (bupd (P' rho) &&
-                        !!(forall rho, RA_normal Q' rho |-- bupd (RA_normal Q rho)) &&
-                        !!(forall rho, RA_break Q' rho |-- bupd (RA_break Q rho)) &&
-                        !!(forall rho, RA_continue Q' rho |-- bupd (RA_continue Q rho)) &&
-                        !!(forall vl rho, RA_return Q' vl rho |-- bupd (RA_return Q vl rho))))
+                   |-- (fupd (P' rho) &&
+                        !!(forall rho, RA_normal Q' rho |-- fupd (RA_normal Q rho)) &&
+                        !!(forall rho, RA_break Q' rho |-- fupd (RA_break Q rho)) &&
+                        !!(forall rho, RA_continue Q' rho |-- fupd (RA_continue Q rho)) &&
+                        !!(forall vl rho, RA_return Q' vl rho |-- fupd (RA_return Q vl rho))))
    (SEM: @semax cs Espec Delta P' c Q'):
    @semax cs Espec Delta P c Q.
 Proof.
