atomics/verif_hashtable_atomic.v
@@ -10,8 +10,6 @@ Require Import VST.atomics.hashtable.
 Require Import VST.msl.iter_sepcon.
 Import List.
 
-Set Bullet Behavior "Strict Subproofs".
-
 #[(*export, after Coq 8.13*)global] Instance CompSpecs : compspecs. make_compspecs prog. Defined.
 Definition Vprog : varspecs. mk_varspecs prog. Defined.
 
